theories/rules/rules_Jmp.v
@@ -79,59 +79,60 @@ Section cap_lang_rules.
     by rewrite Hregs' in Hregs; simplify_eq.
   Qed.
 
-  Definition allow_jmp_mmap_or_true (r : RegName) (regs : Reg) (mem : Mem):=
+  (* NOTE: cond is a condition to re-use the setup with rules_Jnz.v *)
+  Definition allow_jmp_mmap_or_true (cond : Prop) `{Decision cond} (r : RegName) (regs : Reg) (mem : Mem) :=
     ∃ p b e a, read_reg_inr regs r p b e a ∧
-                 if decide (reg_allows_IE_jmp regs r p b e a) then
+                 if decide (reg_allows_IE_jmp regs r p b e a /\ cond) then
                    ∃ w1 w2,
                      mem !! a = Some w1
                      /\ mem !! (a^+1)%a = Some w2
                  else True.
 
-  Definition allow_jmp_rmap_or_true (r : RegName) (regs : Reg) :=
+  Definition allow_jmp_rmap_or_true (cond : Prop) `{Decision cond}  (r : RegName) (regs : Reg) :=
     ∃ p b e a, read_reg_inr regs r p b e a ∧
-                 if decide (reg_allows_IE_jmp regs r p b e a) then
+                 if decide (reg_allows_IE_jmp regs r p b e a /\ cond) then
                    ∃ widc, regs !! idc = Some widc
                  else True.
 
-  Lemma allow_jmp_mmap_or_true_not_ie (r : RegName) (regs : Reg) (mem : Mem) (w : Word) :
+  Lemma allow_jmp_mmap_or_true_not_ie (cond : Prop) `{Decision cond}  (r : RegName) (regs : Reg) (mem : Mem) (w : Word) :
     is_ie_cap w = false ->
     regs !! r = Some w ->
-    allow_jmp_mmap_or_true r regs mem.
+    allow_jmp_mmap_or_true cond r regs mem.
   Proof.
     intros Hvpc.
     destruct_word w; eauto; eexists _,_,_,_; split
     ;try (rewrite /read_reg_inr ; simplify_map_eq; auto).
     rewrite /reg_allows_IE_jmp ; simplify_map_eq ; auto.
     all: case_decide as Heq ; simplify_eq ; auto.
-    all: try destruct Heq as (? & -> & ? & ?) ; simplify_map_eq.
-    all: try destruct Heq as (? & _) ; simplify_map_eq.
+    all: try destruct Heq as [(? & -> & ? & ?) ?] ; simplify_map_eq.
+    all: try destruct Heq as [(? & _) ?] ; simplify_map_eq.
     Unshelve. all: try exact O; try exact 0%a.
   Qed.
 
-  Lemma allow_jmp_rmap_or_true_not_ie (r : RegName) (regs : Reg) (w : Word) :
+  Lemma allow_jmp_rmap_or_true_not_ie (cond : Prop) `{Decision cond}  (r : RegName) (regs : Reg) (w : Word) :
     is_ie_cap w = false ->
     regs !! r = Some w ->
-    allow_jmp_rmap_or_true r regs.
+    allow_jmp_rmap_or_true cond r regs.
   Proof.
     intros Hvpc.
     destruct_word w; eauto; eexists _,_,_,_; split
     ;try (rewrite /read_reg_inr ; simplify_map_eq; auto).
     rewrite /reg_allows_IE_jmp ; simplify_map_eq ; auto.
     all: case_decide as Heq ; simplify_eq ; auto.
-    all: try destruct Heq as (? & -> & ? & ?) ; simplify_map_eq.
-    all: try destruct Heq as (? & _) ; simplify_map_eq.
+    all: try destruct Heq as [(? & -> & ? & ?) ?] ; simplify_map_eq.
+    all: try destruct Heq as [(? & _) ?] ; simplify_map_eq.
     Unshelve. all: try exact O; try exact 0%a.
   Qed.
 
 
-  Lemma allow_jmp_mmap_or_true_ie
+  Lemma allow_jmp_mmap_or_true_ie (cond : Prop) `{Decision cond}
     (r : RegName) (regs : Reg) (mem : Mem)
     (b e a : Addr) (widc wa wa' : Word) :
     regs !! r = Some (WCap IE b e a) ->
     regs !! idc = Some widc ->
     mem !! a = Some wa ->
     mem !! (a ^+1)%a = Some wa' ->
-    allow_jmp_mmap_or_true r regs mem.
+    allow_jmp_mmap_or_true cond r regs mem.
   Proof.
     eexists IE,b,e,a.
     split ; auto.
@@ -141,12 +142,12 @@ Section cap_lang_rules.
     split ; by simplify_map_eq.
   Qed.
 
-  Lemma allow_jmp_rmap_or_true_ie
+  Lemma allow_jmp_rmap_or_true_ie (cond : Prop) `{Decision cond}
     (r : RegName) (regs : Reg)
     (b e a : Addr) (widc : Word) :
     regs !! r = Some (WCap IE b e a) ->
     regs !! idc = Some widc ->
-    allow_jmp_rmap_or_true r regs.
+    allow_jmp_rmap_or_true cond r regs.
   Proof.
     eexists IE,b,e,a.
     split ; auto.
@@ -155,43 +156,74 @@ Section cap_lang_rules.
     eexists _; by simplify_map_eq.
   Qed.
 
-  Lemma allow_jmp_mmap_or_true_ie_fail
+  Lemma allow_jmp_mmap_or_true_ie_fail (cond : Prop) `{Decision cond}
     (r : RegName) (regs : Reg) (mem : Mem)
     (b e a : Addr) (widc wa wa' : Word) :
     not (withinBounds b e a /\ withinBounds b e (a^+1)%a) ->
     regs !! r = Some (WCap IE b e a) ->
-    allow_jmp_mmap_or_true r regs mem.
+    allow_jmp_mmap_or_true cond r regs mem.
   Proof.
     eexists IE,b,e,a.
     split ; auto.
     unfold read_reg_inr; by simplify_map_eq.
     case_decide as Hajmp; auto.
     rewrite /reg_allows_IE_jmp in Hajmp.
-    by destruct Hajmp as ( _ & _ & Hcontra ).
+    by destruct Hajmp as [( _ & _ & Hcontra ) _].
   Qed.
 
-  Lemma allow_jmp_rmap_or_true_ie_fail
+  Lemma allow_jmp_rmap_or_true_ie_fail (cond : Prop) `{Decision cond}
     (r : RegName) (regs : Reg)
     (b e a : Addr) (widc wa wa' : Word) :
     not (withinBounds b e a /\ withinBounds b e (a^+1)%a) ->
     regs !! r = Some (WCap IE b e a) ->
-    allow_jmp_rmap_or_true r regs.
+    allow_jmp_rmap_or_true cond r regs.
   Proof.
     eexists IE,b,e,a.
     split ; auto.
     unfold read_reg_inr; by simplify_map_eq.
     case_decide as Hajmp; auto.
     rewrite /reg_allows_IE_jmp in Hajmp.
-    by destruct Hajmp as ( _ & _ & Hcontra ).
+    by destruct Hajmp as [( _ & _ & Hcontra ) _].
   Qed.
 
+  Lemma allow_jmp_mmap_or_true_false_cond
+    (cond : Prop) `{Decision cond} (r : RegName) (regs : Reg) (mem : Mem)
+    (p : Perm) (b e a : Addr)
+    :
+    read_reg_inr regs r p b e a ->
+    not cond ->
+    allow_jmp_mmap_or_true cond r regs mem.
+  Proof.
+    intros Hrinr Hcond.
+    rewrite /allow_jmp_mmap_or_true.
+    eexists _,_,_,_; split ; eauto.
+    rewrite decide_False //=.
+    by intros [_ ?]; apply Hcond.
+  Qed.
+
+  Lemma allow_jmp_rmap_or_true_false_cond
+    (cond : Prop) `{Decision cond} (r : RegName) (regs : Reg)
+    (p : Perm) (b e a : Addr)
+    :
+    read_reg_inr regs r p b e a ->
+    not cond ->
+    allow_jmp_rmap_or_true cond r regs.
+  Proof.
+    intros Hrinr Hcond.
+    rewrite /allow_jmp_rmap_or_true.
+    eexists _,_,_,_; split ; eauto.
+    rewrite decide_False //=.
+    by intros [_ ?]; apply Hcond.
+  Qed.
+
+  Definition cond_jmp : Prop := True.
   Lemma wp_jmp Ep pc_p pc_b pc_e pc_a r w mem regs  :
     decodeInstrW w = Jmp r →
     isCorrectPC (WCap pc_p pc_b pc_e pc_a) →
 
     regs !! PC = Some (WCap pc_p pc_b pc_e pc_a) →
-    allow_jmp_mmap_or_true r regs mem ->
-    allow_jmp_rmap_or_true r regs ->
+    allow_jmp_mmap_or_true cond_jmp r regs mem ->
+    allow_jmp_rmap_or_true cond_jmp r regs ->
     regs_of (Jmp r) ⊆ dom regs →
     mem !! pc_a = Some w →
 
@@ -250,7 +282,7 @@ Section cap_lang_rules.
 
         case_decide as Hdec ; last simplify_map_eq.
         2: { exfalso; apply Hdec. repeat (split ; auto). }
-        destruct Hdec as (Hreg & _ & _ & _).
+        destruct Hdec as [(Hreg & _ & _ & _) _].
         destruct HallowLoad as (wpc & widc & HaLoad & Ha'Load).
         destruct HallowLoad' as (w' & Hidc).
 
@@ -410,7 +442,7 @@ Section cap_lang_rules.
     iDestruct (map_of_regs_3 with "HPC Hr Hidc") as "[Hreg %Hr']".
     destruct Hr' as (?&?&?).
     iApply (wp_jmp with "[$Hmem $Hreg]"); eauto ; simplify_map_eq; eauto.
-    { eapply (allow_jmp_mmap_or_true_ie _ _ _ _ _ a) ; simplify_map_eq ; eauto. }
+    { eapply (allow_jmp_mmap_or_true_ie _ _ _ _ _ _ a); simplify_map_eq; eauto. }
     { by eapply allow_jmp_rmap_or_true_ie ; simplify_map_eq ; auto. }
     { by rewrite !dom_insert; set_solver+. }
 
@@ -460,7 +492,7 @@ Section cap_lang_rules.
     by simplify_map_eq.
     iDestruct (map_of_regs_2 with "HPC Hidc") as "[Hreg _]".
     iApply (wp_jmp with "[$Hmem $Hreg]"); eauto ; simplify_map_eq; eauto.
-    { eapply (allow_jmp_mmap_or_true_ie _ _ _ _ _ a) ; simplify_map_eq ; eauto. }
+    { eapply (allow_jmp_mmap_or_true_ie _ _ _ _ _ _ a) ; simplify_map_eq ; eauto. }
     { by eapply allow_jmp_rmap_or_true_ie ; simplify_map_eq ; auto. }
     { by rewrite !dom_insert; set_solver+. }
 
@@ -548,7 +580,7 @@ Section cap_lang_rules.
     by simplify_map_eq.
     iDestruct (map_of_regs_2 with "HPC Hidc") as "[Hreg %Hr']".
     iApply (wp_jmp with "[$Hmem $Hreg]"); eauto ; simplify_map_eq; eauto.
-    { eapply (allow_jmp_mmap_or_true_ie _ _ _ _ _ a) ; simplify_map_eq ; eauto. }
+    { eapply (allow_jmp_mmap_or_true_ie _ _ _ _ _ _ a) ; simplify_map_eq ; eauto. }
     { by eapply allow_jmp_rmap_or_true_ie ; simplify_map_eq ; auto. }
     { by rewrite !dom_insert; set_solver+. }
 
